verified fix low blood supply

Dafny/cleanup3/Blood.dfy
@@ -1,10 +1,5 @@
 
-datatype BloodType = AP | BP | OP | ABP | AM | BM | OM | ABM
-
-predicate validBloodType(bloodType: BloodType)
-{
-    bloodType in [AP, BP, OP, ABP, AM, BM, OM, ABM]
-}
+include "BloodType.dfy"
 
 class Blood
 {
