Dafny/cleanup3/BloodType.dfy
@@ -1,0 +1,7 @@
+
+datatype BloodType = AP | BP | OP | ABP | AM | BM | OM | ABM
+
+predicate validBloodType(bloodType: BloodType)
+{
+    bloodType in [AP, BP, OP, ABP, AM, BM, OM, ABM]
+}
